src/provers/LocalsProver.v
@@ -18,45 +18,49 @@ Section LocalsProver.
   Variable funcs' : functions types.
   Definition funcs := Locals.funcs funcs'.
 
-  Definition localsSimplify (e : expr types) : expr types :=
+  Definition localsSimplify (e : expr) : expr :=
     match e with
-      | Func 11 (vs :: Const t nm :: nil) =>
-        match t return tvarD types t -> _ with
-          | tvType 6 => fun nm => sym_sel vs nm
-          | _ => fun _ => e
-        end nm
+      | Func 18 (vs :: nm :: nil) =>
+        match toConst_string nm with
+          | Some nm => sym_sel vs nm
+          | _ => e
+        end
       | _ => e
     end.
 
-  Definition localsProve (_ : unit) (goal : expr types) := 
+  Definition localsProve (_ : unit) (goal : expr) := 
     match goal with
       | Equal _ x y => expr_seq_dec (localsSimplify x) (localsSimplify y)
       | _ => false
     end.
 
-  Lemma localsSimplify_correct : forall uvars vars (e : expr types) t v,
+  Lemma localsSimplify_correct : forall uvars vars (e : expr) t v,
     exprD funcs uvars vars e t = Some v
     -> exprD funcs uvars vars (localsSimplify e) t = Some v.
+  Proof.
     destruct e; simpl; intuition idtac.
-    do 12 (destruct f; try assumption).
-    do 2 (destruct l; try assumption).
-    destruct e0; try assumption.
-    destruct l; try assumption.
-    destruct t0; try assumption.
-    do 7 (destruct n; try assumption).
-    simpl in *.
+    do 19 (destruct f; try assumption).
+    do 3 (destruct l; try assumption).
+    generalize (toConst_string_sound funcs e0).
+    destruct (toConst_string e0); auto.
+    simpl in H.
     destruct (equiv_dec (tvType 0) t); try discriminate.
-    hnf in e0; subst.
-    generalize (sym_sel_correct funcs' uvars vars t1 e).
-    unfold funcs in *.
+    hnf in e1; subst.
+    change ((forall uvars0 vars0 : env (Locals.types types'),
+               exprD funcs uvars0 vars0 e0 (tvType 8) = Some s) ->
+            exprD funcs uvars vars (sym_sel e s) (tvType 0) = Some v).
+    intro.
+    rewrite H0 in *.
+    generalize (sym_sel_correct funcs' uvars vars s e).
+    change (Locals.funcs funcs') with funcs.
     match type of H with
       | match ?E with Some _ => _ | _ => _ end _ _ = _ => destruct E; try discriminate
     end.
-    injection H; clear H; intros; subst.
-    auto.
+    intro X. rewrite <- H. eapply X. reflexivity.
   Qed.
 
   Theorem localsProveCorrect : ProverCorrect funcs reflexivityValid localsProve.
+  Proof.
     unfold localsProve; hnf; simpl; intros.
 
     destruct goal; try discriminate.
@@ -74,11 +78,11 @@ Section LocalsProver.
     congruence.
   Qed.
 
-  Definition localsProver : ProverT types :=
+  Definition localsProver : ProverT :=
     {| Facts := unit
-      ; Summarize := reflexivitySummarize
-      ; Learn := reflexivityLearn
-      ; Prove := localsProve |}.
+     ; Summarize := reflexivitySummarize
+     ; Learn := reflexivityLearn
+     ; Prove := localsProve |}.
 
   Definition localsProver_correct : ProverT_correct localsProver funcs.
     eapply Build_ProverT_correct with (Valid := reflexivityValid : _ -> _ -> Facts localsProver -> Prop); unfold reflexivityValid; eauto.
